feat: Stlc fv

CollapsingTowers/Stlc/SmallStep.lean
@@ -15,7 +15,7 @@ inductive ctx𝕄 : Ctx -> Prop where
   | ctx𝕄_𝔹 : ctx𝔹 B -> ctx𝕄 M -> ctx𝕄 (B ∘ M)
 
 inductive step : Expr -> Expr -> Prop where
-  | step_appβ : ctx𝕄 M -> lc (.lam e) -> value v -> step M⟦.app (.lam e) v⟧ M⟦open₀ e v⟧
+  | step_appβ : ctx𝕄 M -> lc (.lam e) -> value v -> step M⟦.app (.lam e) v⟧ M⟦open₀ v e⟧
 
 inductive mulit : Expr -> Expr -> Prop where
   | multi_stop : mulit e e
@@ -149,3 +149,9 @@ theorem step_deterministic : step expr₀ expr₁ -> step expr₀ expr₂ -> exp
           rw [HEq.left]
           have HEq := IHM₀ HM₁ HEq.right
           rw [HEq]
+
+theorem step_not_value : step e₀ e₁ -> ¬value e₀ :=
+  by
+  intro Hstep Hvalue
+  cases Hstep with
+  | step_appβ HM _ _ => nomatch (ctx𝕄_value HM Hvalue).right
